Refactor Arrow classes and Kappa Calculus (#140)
- Change ex{l,r} to cancel{r,l}, restricting what can be dropped.
Ex{l,r} allowed dropping a value of arbitrary type. Changing to the
stricter cancel{r,l} which only allows discarding a term of unit type is
a step towards the correct generalized arrow class hierarchy.

- Add Arrows laws

- Split Arrow into Copy Drop Swap Arrow classes

- Move circuit equivalences to dedicated class

- Merge delay into Cava and add ArrowLoop as a subclass

- Revert Arrow.Cava methods to not have rightmost unit

- Update kappa_sugared to include all Cava methods

- Update arrow-examples and remove concatenative examples

cava/arrow-examples/ArrowExamplesSV.hs
@@ -19,17 +19,10 @@ module Main where
 import Cava2SystemVerilog
 import Mux2_1
 import ArrowAdder
-import Examples
 import SyntaxExamples
 
 main :: IO ()
-main = do writeSystemVerilog nandArrow
-          writeTestBench arrow_nand2_tb
-          writeSystemVerilog xorArrow
-          writeTestBench arrow_xor_tb
-          writeSystemVerilog feedbackNandArrow
-          writeTestBench feedbackNandArrow_tb
-          writeSystemVerilog mux2_1_netlist
+main = do writeSystemVerilog mux2_1_netlist
           writeTestBench mux2_1_tb
           writeSystemVerilog fullAdder_netlist
           writeTestBench fullAdder_tb
