cava/cava/Cava/Arrow/Kappa/Syntax.v
@@ -1,137 +1,210 @@
-Require Export Cava.Arrow.Kappa.Kappa.
-Require Export Cava.Arrow.Kappa.CC.
-Require Export Cava.Arrow.Instances.Combinational.
-Require Export Cava.Arrow.Instances.Constructive.
+Require Import Arith Eqdep_dec List Lia NArith.
 
-Require Import Cava.Types.
-Require Import Cava.Arrow.Arrow.
 Require Import Cava.BitArithmetic.
 
-Require Import Arith Eqdep_dec List Lia Program.
+Require Import Cava.Arrow.Arrow.
+Require Export Cava.Arrow.Instances.Constructive.
+Require Export Cava.Arrow.Kappa.Kappa.
+Require Export Cava.Arrow.Kappa.CC.
 
 (* Notations *)
 
 Require Import List Lia.
 Import ListNotations.
 
-Declare Scope expression_scope.
+Declare Scope kappa_scope.
 Declare Custom Entry expr.
-Delimit Scope expression_scope with source.
+Delimit Scope kappa_scope with kappa.
 
-Notation "<[ e ]>" := (
-  Desugar (fun var =>
-    e%source
-  )
-  ) (at level 1, e custom expr at level 1).
+(* Kappa expression and application *)
+Module KappaNotation.
+  Notation "<[ e ]>" := (fun var => e%kappa) (at level 1, e custom expr at level 1).
 
-Notation "\ x .. y => e" := (Abs (fun x => .. (Abs (fun y => e)) ..))
-  (in custom expr at level 200, x binder, right associativity,
-   format "'[' \  '/  ' x  ..  y =>  '/  ' e ']'")
-                                  : expression_scope.
+  Notation "\ x .. y => e" := (Abs (fun x => .. (Abs (fun y => e)) ..))
+    (in custom expr at level 200, x binder, right associativity,
+    format "'[' \  '/  ' x  ..  y =>  '/  ' e ']'")
+                                    : kappa_scope.
 
-Notation "x y" := (App x y) (in custom expr at level 3, left associativity) : expression_scope.
-Notation "~~( x )" := (Arr x) (in custom expr, x constr) : expression_scope.
+  Notation "x y" := (App x y) (in custom expr at level 3, left associativity) : kappa_scope.
 
-Notation "! x" := ( (Arr x)) (in custom expr at level 2, x global) : expression_scope.
+  Notation "x" := (Var x) (in custom expr, x ident) : kappa_scope.
+  Notation "( x )" := x (in custom expr, x at level 4) : kappa_scope.
+  Notation "'let' x = e1 'in' e2" := (Let e1 (fun x => e2)) (in custom expr at level 1, x constr at level 4, e2 at level 5, e1 at level 1) : kappa_scope.
 
-Notation "~!( x )" := (Arr (Closure_conversion x)) (in custom expr, x constr) : expression_scope.
-
-Notation "'let' x = e1 'in' e2" := (Let e1 (fun x => e2)) (in custom expr at level 1, x constr at level 4, e2 at level 5, e1 at level 1) : expression_scope.
-Notation "x" := (Var x) (in custom expr, x ident) : expression_scope.
-Notation "( x )" := x (in custom expr, x at level 4) : expression_scope.
-
-Notation "( x , y )" := (
-    Com (Arr (unassoc >>> exl)) (App (App (Arr id) x) y)
+  (* todo: turn into a recursive pattern *)
+  Notation "'let' '( x , y ) = e1 'in' e2"
+    := (
+    Let (App TupleLeft e1) (fun x => 
+      Let (App TupleRight e1) (fun y => e2
+      )
     )
-   (in custom expr, x at level 4, y at level 4) : expression_scope.
+    ) 
+    (in custom expr at level 1, x constr at level 4, y constr at level 4, e2 at level 5, e1 at level 1) : kappa_scope.
 
-Notation "'fst'' e" := (Com (Arr exl) e) (in custom expr at level 4, e custom expr at level 4) : expression_scope.
-Notation "'snd'' e" := (Com (Arr exr) e) (in custom expr at level 4, e custom expr at level 4) : expression_scope.
+  (* Escaping *)
 
-Notation "# x" := (Arr (constant x)) (in custom expr at level 2, x constr at level 4) : expression_scope.
-Notation "#v x" := (Arr (constant_vec _ x)) (in custom expr at level 2, x constr at level 4) : expression_scope.
+  Notation "! x" := (x _)(in custom expr at level 2, x global) : kappa_scope.
+  Notation "!( x )" := (x _) (in custom expr, x constr) : kappa_scope.
+
+  Notation "( x , .. , y , z )" := (
+    (tupleHelper x .. (tupleHelper y z) .. )
+    )
+    (in custom expr, x at level 4, y at level 4, z at level 4) : kappa_scope.
+
+  (* Pre defined functions *)
+
+  Notation "'fst'" := (TupleLeft) (in custom expr at level 4) : kappa_scope.
+  Notation "'snd'" := (TupleRight) (in custom expr at level 4) : kappa_scope.
+
+  Notation "'not'" := (Not) (in custom expr at level 4) : kappa_scope.
+  Notation "'and'" := (And) (in custom expr at level 4) : kappa_scope.
+  Notation "'nand'" := (Nand) (in custom expr at level 4) : kappa_scope.
+  Notation "'or'" := (Or) (in custom expr at level 4) : kappa_scope.
+  Notation "'nor'" := (Nor) (in custom expr at level 4) : kappa_scope.
+  Notation "'xor'" := (Xor) (in custom expr at level 4) : kappa_scope.
+  Notation "'xnor'" := (Xnor) (in custom expr at level 4) : kappa_scope.
+  Notation "'buf'" := (Buf) (in custom expr at level 4) : kappa_scope.
+  Notation "'delay'" := (Delay) (in custom expr at level 4) : kappa_scope.
+
+  Notation "'xorcy'" := (Xorcy) (in custom expr at level 4) : kappa_scope.
+  Notation "'muxcy'" := (Muxcy) (in custom expr at level 4) : kappa_scope.
+  Notation "'unsigned_add'" := (UnsignedAdd _ _ _) (in custom expr at level 4) : kappa_scope.
+
+  Notation "'index_vec'" := (IndexVec _) (in custom expr at level 4) : kappa_scope.
+  Notation "'to_vec'" := (ToVec) (in custom expr at level 4) : kappa_scope.
+  Notation "'concat'" := (Concat _) (in custom expr at level 4) : kappa_scope.
+
+  Notation "'true'" := (Constant true) (in custom expr at level 2) : kappa_scope.
+  Notation "'false'" := (Constant false) (in custom expr at level 2) : kappa_scope.
+
+  Notation "# x" := (ConstantVec x) (in custom expr at level 2, x constr at level 4) : kappa_scope.
+
+  Notation "x [ v ]" := (App (App (IndexVec _) x) v) (in custom expr at level 4) : kappa_scope.
+End KappaNotation.
+
+Definition to_constructive {i o} (expr: Kappa i o) (wf: wf_debrujin ENil (expr _))
+  : structure (remove_rightmost_unit i) o
+  := Compose (closure_conversion expr wf) (insert_rightmost_tt1 _) .
+Definition compile_kappa {i o} (Cava: Cava) (expr: Kappa i o) (wf: wf_debrujin ENil (expr _))
+  : denoteKind (remove_rightmost_unit i) ~> denoteKind o 
+  := toCava Cava (to_constructive expr wf).
+
+Ltac auto_kappa_wf := simpl;tauto.
+
+Ltac build_structure kappa_term :=
+    let reduced := eval compute in (to_constructive (Desugar kappa_term) (ltac:(auto_kappa_wf))) 
+    in exact reduced.
 
 (* test notation *)
 
-Local Open Scope expression_scope.
+Section regression_examples.
+  Import KappaNotation.
+  Local Open Scope kappa_scope.
 
-(* 1. simple constant *)
-Definition ex1_notation: Kappa << bit >> bit := <[ \ x => #true ]> .
+  Definition ex1_constant: Kappa_sugared << Bit, Unit >> Bit := <[ \x => true ]>.
+  Definition ex2_parameterized (n:nat) : Kappa_sugared << Bit, Unit >> Bit :=
+  match n with
+  | O => <[ \ x => true ]>
+  | S n => <[ \ x => xor x x ]>
+  end.
 
-(* 2. branching on Coq value *)
-Definition ex2_notation (n:nat) : Kappa << bit >> bit :=
-match n with
-| O => <[ \ x => #true ]>
-| S n => <[ \ x => !xor_gate x x ]>
-end.
+  Definition ex3_to_vec: Kappa_sugared << Bit, Unit >>  (Vector 1 Bit) :=
+  <[ \ x => to_vec x ]>.
+  Definition ex4_index_vec: Kappa_sugared << Vector 10 Bit, Unit >> Bit :=
+  <[ \ x => index_vec x (# 1) ]>.
+  Definition ex5_index_vec2: Kappa_sugared << Vector 10 Bit, Unit >> Bit :=
+  <[ \ x => x [# 1] ]>.
+  Definition ex6_concat: Kappa_sugared << Vector 2 Bit, Bit, Unit >> (Vector 3 Bit) :=
+  <[ \ x v => concat x v ]>.
+  Definition ex7_xor: Kappa_sugared << Bit, Bit, Unit >> Bit := 
+  <[ \ x y => xor x y ]>.
+  Definition ex7_tupled_destruct: Kappa_sugared << << Bit, Bit>>, Unit>> Bit := 
+  <[ \ xy => 
+    let '(x,y) = xy in
+    y ]>.
+  Definition ex8_multiindex: Kappa_sugared << Vector 10 (Vector 5 Bit), Unit >> Bit :=
+  <[ \ x => x[#0][#1] ]>.
 
-(* 3. adder tree *)
-Fixpoint make_obj o (n:nat): bundle :=
-match n with
-| O => o
-| S n => Tuple2 (make_obj o n) (make_obj o n)
-end.
+  Fixpoint copy_object_pow2 o (n:nat): Kind :=
+  match n with
+  | O => o
+  | S n => Tuple (copy_object_pow2 o n) (copy_object_pow2 o n)
+  end.
 
-Fixpoint tree (A: object)
-  (n: nat)
-  (f: << A, A >> ~> A)
-  {struct n}
-  : Kappa (make_obj A n ** unit) A :=
-match n with
-| O => <[ \x => x ]>
-| S n' => <[\x =>
-            let a = ~!(tree A n' f) (fst' x) in
-            let b = ~!(tree A n' f) (snd' x) in
+  Fixpoint tree 
+    (A: Kind)
+    (n: nat)
+    (f:  Kappa_sugared << A, A, Unit >> A)
+    {struct n}
+    : Kappa_sugared << copy_object_pow2 A n, Unit >> A :=
+  match n with
+  | O => <[ \x => x ]>
+  | S n' =>
+    <[\ x =>
+        let a = !(tree A n' f) (fst x) in
+        let b = !(tree A n' f) (snd x) in
+        !f a b
+    ]>
+  end.
 
-            !f a b
-            ]>
-end.
+  Definition xilinxFullAdder
+    : Kappa_sugared << Bit, << Bit, Bit >>, Unit>> (Tuple Bit Bit) :=
+    <[ \ cin ab =>
+      let a = fst ab in
+      let b = snd ab in
+      let part_sum = xor a b in
+      let sum      = xorcy part_sum cin in
+      let cout     = muxcy part_sum (cin, a) in
+      (sum, cout)
+    ]>.
 
-Definition xilinxFullAdder
-  : Kappa << bit, bit ** bit >> (bit**bit) :=
-  <[ \ cin ab =>
-     let a = fst' ab in
-     let b = snd' ab in
-     let part_sum = !xor_gate a b in
-     let sum      = !xorcy part_sum cin in
-     let cout     = !muxcy part_sum (cin, a) in
-     (sum, cout)
-  ]>.
+  Definition adder_tree
+    (bitsize: N)
+    (n: nat)
+    : Kappa_sugared (copy_object_pow2 (Vector bitsize Bit) n ** unit) (Vector bitsize Bit) :=
+    tree (Vector bitsize Bit) n (fun var => UnsignedAdd _ _ _).
 
-Definition adder_tree
-  (bitsize: nat)
-  (n: nat)
-  : Kappa (make_obj (bitvec [bitsize]) n ** unit) (bitvec [bitsize]) :=
-  tree (bitvec [bitsize]) n (unsigned_add _ _ _).
+End regression_examples.
 
-Lemma kappa_arrow_lemma_example:
+(* Lemma kappa_arrow_lemma_example:
   forall (Cava: Cava),
-  toCava _ (Closure_conversion ex1_notation) = 
-  (uncancelr >>> first swap >>> assoc >>> exl >>> constant true).
+  compile_kappa _ ex1_notation = drop >>> constant true.
+  (* (uncancelr >>> first swap >>> assoc >>> cancelr >>> constant true). *)
 Proof.
   intros.
+  cbv [compile_kappa toCava to_constructive ex1_notation].
+  simpl.
+
   auto.
-Qed.
+Abort.
 
 Ltac simpl_conversion :=
   cbv beta iota zeta delta [
     Desugar desugar Closure_conversion closure_conversion closure_conversion'
-    as_object_list  object_to_list_object_id  extract_nth'
+    extract_nth'
     wf_debrujin_succ
     eq_rec_r eq_rec eq_rect eq_rect_r eq_ind_r eq_ind eq_sym f_equal
     length
-    as_object_is_as_list_as_object Nat.eq_dec
+    Nat.eq_dec
     nat_rec nat_rect environment_ind eq_trans
+    to_constructive
+    ConstructiveCava
+    ConstructiveCat
+    ConstructiveArr
+    morphism
+    compose
+    (* uncancelr *)
   ].
 
 Lemma kappa_arrow_lemma_example2:
-  Closure_conversion ex1_notation =M= (drop >>> constant true).
+  to_constructive ex1_notation =M= (drop >>> constant true).
 Proof.
   intros.
   unfold ex1_notation.
   simpl_conversion.
+  fold (@cancelr _ unit).
 
-  setoid_rewrite exl_unit_is_drop.
+  setoid_rewrite cancelr_unit_is_drop.
   setoid_rewrite <- associativity at 1.
   setoid_rewrite <- associativity at 1.
   setoid_rewrite <- associativity at 1.
@@ -144,11 +217,11 @@ Definition xilinxFullAdderWf: (wf_debrujin ENil (xilinxFullAdder _)).
 Defined.
 
 Goal
-  structural_simplification (closure_conversion xilinxFullAdder xilinxFullAdderWf >>> exl) =M= second (first (second uncancelr >>> xor_gate)) >>> xorcy.
+  structural_simplification (closure_conversion xilinxFullAdder xilinxFullAdderWf >>> cancelr) =M= second (first (second uncancelr >>> xor_gate)) >>> xorcy.
 Proof.
   intros.
   unfold xilinxFullAdder, xilinxFullAdderWf.
   simpl_conversion.
 
   (*TODO*)
-Abort.
+Abort. *)
